erasure/theories/ESpineView.v
@@ -1,0 +1,52 @@
+(* Distributed under the terms of the MIT license. *)
+Require Import List ssreflect ssrbool.
+From MetaCoq.Template Require Import utils BasicAst.
+From MetaCoq.Erasure Require Import EAst EAstUtils EInduction EReflect.
+From MetaCoq.PCUIC Require Import PCUICSize.
+From Equations Require Import Equations.
+Set Equations Transparent.
+
+Module TermSpineView.
+
+Inductive t : term -> Set :=
+| tBox       : t EAst.tBox
+| tRel (n : nat) : t (EAst.tRel n)
+| tVar (n : ident) : t (EAst.tVar n)
+| tEvar (n : nat) (e : list term) : t (EAst.tEvar n e)
+| tLambda n b : t (EAst.tLambda n b)
+| tLetIn n b b' : t (EAst.tLetIn n b b')
+| tApp (f : term) (l : list term) (napp : ~~ isApp f) (nnil : l <> nil) : t (mkApps f l)
+| tConst kn : t (tConst kn)
+| tConstruct i n : t (tConstruct i n)
+| tCase ci p brs : t (tCase ci p brs)
+| tProj p c : t (tProj p c)
+| tFix mfix idx : t (tFix mfix idx)
+| tCoFix mfix idx : t (tCoFix mfix idx).
+Derive Signature for t.
+
+Definition view : forall x : term, t x :=
+  MkAppsInd.rec (P:=fun x => t x)
+    tBox tRel tVar 
+    (fun n l _ => tEvar n l) 
+    (fun n t _ => tLambda n t)
+    (fun n b _ t _ => tLetIn n b t)
+    (fun f l napp nnil _ _ => tApp f l napp nnil)
+    tConst
+    tConstruct
+    (fun p t pt l pl => tCase p t l)
+    (fun p t pt => tProj p t)
+    (fun mfix n _ => tFix mfix n)
+    (fun mfix n _ => tCoFix mfix n).
+
+Lemma view_mkApps {f v} (vi : t (mkApps f v)) : ~~ isApp f -> v <> [] -> 
+  exists hf vn, vi = tApp f v hf vn.
+Proof.
+  intros ha hv.
+  depelim vi.
+  all: try (revert H; eapply DepElim.simplification_sigma1; intros H'; solve_discr).
+  intros He.
+  epose proof (DepElim.pr2_uip (A:=EAst.term) He). subst vi0.
+  do 2 eexists; reflexivity.
+Qed.
+  
+End TermSpineView.
